examples/Nimp.v
@@ -155,7 +155,7 @@ Qed.
 (* SAZ: the [~] notation for eutt wasn't working here. *)
 Lemma eval_one_loop : eval one_loop ≈ one_loop_tree.
 Proof.
-  einit. ecofix CIH.
+  einit. ecofix CIH. edrop.
   setoid_rewrite rec_as_interp.
   setoid_rewrite interp_bind.
   setoid_rewrite interp_vis.
@@ -164,13 +164,12 @@ Proof.
   setoid_rewrite bind_bind.
   setoid_rewrite bind_ret.
   setoid_rewrite bind_vis.
-  evis. intros. 
+  evis. intros.
   setoid_rewrite bind_ret.
   destruct v.
   - setoid_rewrite interp_ret. apply reflexivity.
   - setoid_rewrite interp_bind.
     setoid_rewrite interp_recursive_call.
-    setoid_rewrite tau_eutt.
     setoid_rewrite eval_skip.
     setoid_rewrite bind_ret.
     eauto with paco.
