theories/Core/KTreeFacts.v
@@ -29,66 +29,78 @@ Local Open Scope itree.
 
 (** ** [ITree.aloop] *)
 
-Lemma bind_aloop {E A B C} (f : A -> itree E A + B) (g : B -> itree E B + C): forall x,
-    (ITree.aloop f x >>= ITree.aloop g)
-  ≈ ITree.aloop (fun ab =>
+Lemma bind_iter {E A B C} (f : A -> itree E (A + B)) (g : B -> itree E (B + C))
+  : forall x,
+    (ITree.iter f x >>= ITree.iter g)
+  ≈ ITree.iter (fun ab =>
        match ab with
-       | inl a => inl (ITree._aloop id (fun a => Ret (inl a))
-                                    (bimap (id_ _) inr (f a)))
-       | inr b => apply_Fun (bimap (ITree.map inr) (id_ _)) (g b)
+       | inl a => ITree.map inl (f a)
+       | inr b => ITree.map (bimap inr (id_ _)) (g b)
        end) (inl x).
 Proof.
   einit. ecofix CIH. intros.
-  rewrite !unfold_aloop. unfold ITree._aloop.
-  destruct (f x) as [t | b]; cbn.
-  - unfold id. rewrite bind_tau. etau. rewrite !bind_bind.
-    ebind. econstructor; try reflexivity.
-    intros. subst. rewrite bind_ret. eauto with paco.
-  - rewrite bind_ret, tau_eutt, bind_ret.
+  rewrite !unfold_iter. unfold ITree._iter.
+  rewrite bind_map, bind_bind.
+  ebind; econstructor; try reflexivity.
+  intros [a | b] _ [].
+  - rewrite bind_tau. etau.
+  - rewrite bind_ret, tau_eutt.
     revert b. ecofix CIH'. intros.
-    rewrite !unfold_aloop. unfold ITree._aloop.
-    destruct (g b) as [t' | c]; cbn; eauto with paco.
-    rewrite bind_map. etau.
-    ebind. econstructor; try reflexivity.
-    intros. subst. eauto with paco.
+    rewrite !unfold_iter. unfold ITree._iter.
+    rewrite bind_map.
+    ebind; econstructor; try reflexivity.
+    intros [b' | c] _ []; cbn.
+    + etau.
+    + reflexivity.
 Qed.
 
-Lemma eq_itree_aloop' {E I1 I2 R1 R2}
+Lemma eq_itree_iter' {E I1 I2 R1 R2}
       (RI : I1 -> I2 -> Prop)
       (RR : R1 -> R2 -> Prop)
-      (body1 : I1 -> itree E I1 + R1)
-      (body2 : I2 -> itree E I2 + R2)
+      (body1 : I1 -> itree E (I1 + R1))
+      (body2 : I2 -> itree E (I2 + R2))
       (eutt_body
-       : forall j1 j2, RI j1 j2 -> sum_rel (eq_itree RI) RR (body1 j1) (body2 j2))
+       : forall j1 j2, RI j1 j2 -> eq_itree (sum_rel RI RR) (body1 j1) (body2 j2))
   : forall (i1 : I1) (i2 : I2) (RI_i : RI i1 i2),
-    @eq_itree E _ _ RR (ITree.aloop body1 i1) (ITree.aloop body2 i2).
+    @eq_itree E _ _ RR (ITree.iter body1 i1) (ITree.iter body2 i2).
 Proof.
   ginit. gcofix CIH. intros.
   specialize (eutt_body i1 i2 RI_i).
-  do 2 rewrite unfold_aloop.
-  destruct eutt_body; cbn; eauto with paco.
-  gstep. econstructor. guclo eqit_clo_bind.
-  gstep. constructor; eauto.
+  do 2 rewrite unfold_iter.
+  guclo eqit_clo_bind; econstructor; eauto.
+  intros ? ? []; gstep; econstructor; auto with paco.
 Qed.
 
-Lemma eutt_aloop' {E I1 I2 R1 R2}
+Lemma eutt_iter' {E I1 I2 R1 R2}
       (RI : I1 -> I2 -> Prop)
       (RR : R1 -> R2 -> Prop)
-      (body1 : I1 -> itree E I1 + R1)
-      (body2 : I2 -> itree E I2 + R2)
+      (body1 : I1 -> itree E (I1 + R1))
+      (body2 : I2 -> itree E (I2 + R2))
       (eutt_body
-       : forall j1 j2, RI j1 j2 -> sum_rel (eutt RI) RR (body1 j1) (body2 j2))
+       : forall j1 j2, RI j1 j2 -> eutt (sum_rel RI RR) (body1 j1) (body2 j2))
   : forall (i1 : I1) (i2 : I2) (RI_i : RI i1 i2),
-    @eutt E _ _ RR (ITree.aloop body1 i1) (ITree.aloop body2 i2).
+    @eutt E _ _ RR (ITree.iter body1 i1) (ITree.iter body2 i2).
 Proof.
   einit. ecofix CIH. intros.
   specialize (eutt_body i1 i2 RI_i).
-  do 2 rewrite unfold_aloop.
-  destruct eutt_body; cbn; eauto with paco.
-  etau. ebind. econstructor; eauto with paco.
+  do 2 rewrite unfold_iter.
+  ebind; econstructor; eauto with paco.
+  intros ? ? [].
+  - etau.
+  - eauto with paco.
 Qed.
 
 (** ** [iter] *)
+
+Lemma eqit_mon {E R1 R2} (RR RR' : R1 -> R2 -> Prop) b1 b2 :
+  (RR <2= RR') ->
+  (eqit RR b1 b2 <2= @eqit E _ _ RR' b1 b2).
+Proof.
+  intros.
+  eapply paco2_mon_bot; eauto.
+  intros ? ? ?. red.
+  induction 1; auto.
+Qed.
 
 Instance eq_itree_iter {E A B} :
   @Proper ((A -> itree E (A + B)) -> A -> itree E B)
@@ -96,9 +108,10 @@ Instance eq_itree_iter {E A B} :
           iter.
 Proof.
   intros body1 body2 EQ_BODY a. repeat red in EQ_BODY.
-  unfold iter, Iter_ktree.
-  eapply (eq_itree_aloop' eq).
-  intros [] ? []; constructor; auto. reflexivity.
+  unfold iter, Iter_Kleisli.
+  eapply (eq_itree_iter' eq); auto.
+  intros; eapply eqit_mon, EQ_BODY; auto.
+  intros [] _ []; auto.
 Qed.
 
 Instance eutt_iter {E A B} :
@@ -107,9 +120,10 @@ Instance eutt_iter {E A B} :
           iter.
 Proof.
   intros body1 body2 EQ_BODY a. repeat red in EQ_BODY.
-  unfold iter, Iter_ktree.
-  eapply (eutt_aloop' eq).
-  intros [] ? []; constructor; auto. reflexivity.
+  unfold iter, Iter_Kleisli.
+  eapply (eutt_iter' eq); auto.
+  intros ? _ []; eapply eqit_mon, EQ_BODY; auto.
+  intros [] _ []; auto.
 Qed.
 
 Definition eutt_iter_gen {F A B R S} :
@@ -119,10 +133,7 @@ Definition eutt_iter_gen {F A B R S} :
 Proof.
   do 3 red;
   intros body1 body2 EQ_BODY x y Hxy. red in EQ_BODY.
-  unfold iter, Iter_ktree.
-  eapply (eutt_aloop' (sum_rel R S)); intros.
-  - destruct H; constructor; auto.
-  - constructor; auto.
+  eapply eutt_iter'; eauto.
 Qed.
 
 Instance eq2_ktree_iter {E A B} :
@@ -131,31 +142,28 @@ Instance eq2_ktree_iter {E A B} :
           iter.
 Proof. apply eutt_iter. Qed.
 
-Section KTreeConway.
+Section KTreeIterative.
 
 Lemma unfold_iter_ktree {E A B} (f : ktree E A (A + B)) (a0 : A) :
-  iter f a0 ≅ Tau (
+  iter f a0 ≅
     ab <- f a0 ;;
     match ab with
-    | inl a => iter f a
+    | inl a => Tau (iter f a)
     | inr b => Ret b
-    end).
+    end.
 Proof.
-  unfold iter, Iter_ktree, cat.
-  rewrite unfold_aloop; cbn.
-  pstep; constructor; left.
+  unfold iter, Iter_Kleisli, Basics.iter, MonadIter_itree, cat.
+  rewrite unfold_iter; cbn.
   eapply eqit_bind; try reflexivity.
-  intros [].
-  reflexivity.
-  rewrite unfold_aloop; cbn.
-  reflexivity.
 Qed.
 
 Instance IterUnfold_ktree {E} : IterUnfold (ktree E) sum.
 Proof.
   repeat intro.
-  rewrite unfold_iter_ktree, tau_eutt.
-  reflexivity.
+  rewrite unfold_iter_ktree.
+  do 2 red. unfold cat, Cat_Kleisli; cbn.
+  eapply eutt_clo_bind; try reflexivity.
+  intros [] ? []; try rewrite tau_eutt; reflexivity.
 Qed.
 
 Instance IterNatural_ktree {E} : IterNatural (ktree E) sum.
@@ -166,17 +174,12 @@ Proof.
   revert a0.
   einit. ecofix CIH. intros.
   rewrite 2 unfold_iter_ktree.
-  rewrite bind_tau.
-  estep; econstructor.
   rewrite !bind_bind.
   ebind; econstructor; try reflexivity.
   intros [] ? [].
-  rewrite 2 bind_ret.
-  eauto with paco.
-  rewrite bind_bind.
-  setoid_rewrite bind_ret.
-  rewrite bind_ret2.
-  reflexivity.
+  - rewrite bind_tau, 2 bind_ret. etau.
+  - rewrite bind_ret, !bind_bind. setoid_rewrite bind_ret. rewrite bind_ret2.
+    reflexivity.
 Qed.
 
 Lemma iter_dinatural_ktree {E A B C}
@@ -187,22 +190,20 @@ Lemma iter_dinatural_ktree {E A B C}
       | inl c => Tau (g c)
       | inr b => Ret (inr b)
       end) a0
-  ≅ Tau (
-       cb <- f a0 ;;
-       match cb with
-       | inl c0 => iter (fun c =>
+  ≅ cb <- f a0 ;;
+     match cb with
+     | inl c0 => Tau (iter (fun c =>
          ab <- g c ;;
          match ab with
          | inl a => Tau (f a)
          | inr b => Ret (inr b)
-         end) c0
-       | inr b => Ret b
-       end).
+         end) c0)
+     | inr b => Ret b
+     end.
 Proof.
   revert A B C f g a0.
   ginit. gcofix CIH. intros.
   rewrite unfold_iter_ktree.
-  gstep; econstructor.
   rewrite bind_bind.
   guclo eqit_clo_bind. econstructor. try reflexivity.
   intros [] ? [].
@@ -211,16 +212,14 @@ Proof.
     rewrite unfold_iter_ktree.
     gstep; econstructor.
     rewrite bind_bind.
-    guclo eqit_clo_bind. econstructor. try reflexivity.
+    guclo eqit_clo_bind; econstructor; try reflexivity.
     intros [] ? [].
-    { rewrite bind_tau.
+    * rewrite bind_tau.
+      gstep; constructor.
       eauto with paco.
-    }
-    { rewrite bind_ret. gstep; econstructor; auto.
-    }
+    * rewrite bind_ret. gstep; econstructor; auto.
   }
-  { rewrite bind_ret. gstep; constructor; auto.
-  }
+  { rewrite bind_ret. gstep; constructor; auto. }
 Qed.
 
 Instance IterDinatural_ktree {E} : IterDinatural (ktree E) sum.
@@ -241,11 +240,11 @@ Proof.
     rewrite tau_eutt; reflexivity.
     reflexivity.
   - rewrite iter_dinatural_ktree.
-    rewrite tau_eutt.
     eapply eutt_clo_bind.
     reflexivity.
     intros [] ? [].
-    + apply eutt_iter; intros x.
+    + rewrite tau_eutt.
+      apply eutt_iter; intros x.
       eapply eutt_clo_bind.
       reflexivity.
       intros [] ? [].
@@ -256,32 +255,35 @@ Qed.
 
 Lemma iter_codiagonal_ktree {E A B} (f : ktree E A (A + (A + B))) (a0 : A)
   : iter (iter f) a0
-  ≅ Tau (iter (fun a =>
+  ≅ iter (fun a =>
        r <- f a ;;
        match r with
        | inl a' => Ret (inl a')
-       | inr (inl a') => Tau (Ret (inl a'))
+       | inr (inl a') => Ret (inl a')
        | inr (inr b) => Ret (inr b)
-       end) a0).
+       end) a0.
 Proof.
   revert a0.
   ginit. gcofix CIH. intros.
   rewrite unfold_iter_ktree.
   rewrite (unfold_iter_ktree (fun _ => _ _ _)).
-  gstep; constructor.
-  revert a0.
-  gcofix CIH'. intros.
-  rewrite bind_bind.
-  rewrite unfold_iter_ktree.
-  rewrite bind_tau, bind_bind.
-  gstep; constructor.
+  rewrite unfold_iter_ktree, !bind_bind.
   guclo eqit_clo_bind. econstructor. reflexivity.
   intros [| []] ? [].
-  - rewrite bind_ret.
+  - rewrite bind_ret, bind_tau.
+    gstep. constructor.
+    revert a.
+    gcofix CIH'. intros.
+    rewrite unfold_iter_ktree.
     rewrite (unfold_iter_ktree (fun _ => _ _ _)).
-    auto with paco.
-  - rewrite bind_tau, 2 bind_ret.
-    auto with paco.
+    rewrite !bind_bind.
+    guclo eqit_clo_bind. econstructor. reflexivity.
+    intros [| []] ? [].
+    + rewrite bind_tau, bind_ret. gstep; constructor; auto with paco.
+    + rewrite 2 bind_ret. gstep; constructor; auto with paco.
+    + rewrite 2 bind_ret. gstep; constructor; auto.
+  - rewrite 2 bind_ret.
+    gstep; constructor; auto with paco.
   - rewrite 2 bind_ret.
     gstep; reflexivity.
 Qed.
@@ -292,7 +294,6 @@ Proof.
   unfold bimap, Bimap_Coproduct, case_, CoprodCase_Kleisli, case_sum, cat, Cat_Kleisli.
   cbn.
   rewrite iter_codiagonal_ktree.
-  rewrite tau_eutt.
   apply eutt_iter.
   intros a1.
   eapply eutt_clo_bind.
@@ -300,9 +301,9 @@ Proof.
   intros [| []] ? []; rewrite ?tau_eutt; reflexivity.
 Qed.
 
-Global Instance Conway_ktree {E} : Conway (ktree E) sum.
+Global Instance Iterative_ktree {E} : Iterative (ktree E) sum.
 Proof.
   split; typeclasses eauto.
 Qed.
 
-End KTreeConway.
+End KTreeIterative.
